iris/ProofUsertrap.v
@@ -1185,13 +1185,21 @@ Lemma usertrap_res_bare_norm
   usertrap_res_bare pt ksp -∗ usertrap_res_bare (ud_norm pt) ksp.
 Proof. exact (ut_res_bare_norm SY.syscall_env pt ksp). Qed.
 
+Lemma usertrap_res_bare_ctx
+    `{!riscvGS Σ, !xv6G Σ, !bioslotG Σ, !fdslotG Σ, !fileG Σ, !irefslotG Σ, !pavG Σ} `{GEN : GenId} `{CID : CpuId} `{XI : CurCtx} (pt : uptd) (ksp : mword 64) :
+  usertrap_res_bare pt ksp -∗
+  own_context cur_ctx ∗ (own_context cur_ctx -∗ usertrap_res_bare pt ksp).
+Proof. exact (ut_res_bare_ctx_acc SY.syscall_env pt ksp). Qed.
+
 Lemma usertrap_res_tf_open
     `{!riscvGS Σ, !xv6G Σ, !bioslotG Σ, !fdslotG Σ, !fileG Σ, !irefslotG Σ, !pavG Σ} `{GEN : GenId} `{CID : CpuId} `{XI : CurCtx} (pt : uptd) (ksp : mword 64) :
   usertrap_res_bare pt ksp -∗
   ∃ (kroot : mword 44) (ws : list (mword 64)),
     kpt_inv kroot ∗ ⌜tf_kernel_words_ok kroot ksp ws⌝ ∗ tf_page (ud_tfp pt) ws ∗
+        own_context cur_ctx ∗
     (∀ ws' : list (mword 64),
        ⌜tf_kernel_words_ok kroot ksp ws'⌝ -∗ tf_page (ud_tfp pt) ws' -∗
+         own_context cur_ctx -∗
        usertrap_res_bare pt ksp).
 Proof. exact (ut_res_bare_tf_open SY.syscall_env pt ksp). Qed.
 
@@ -1221,9 +1229,9 @@ Lemma usertrap_res_tf_csrs_open
   usertrap_res_bare pt ksp -∗
   ∃ (kroot : mword 44) (ws : list (mword 64)),
     kpt_inv kroot ∗ ⌜tf_kernel_words_ok kroot ksp ws⌝ ∗
-    tf_page (ud_tfp pt) ws ∗ hart_csrs ∗
+    tf_page (ud_tfp pt) ws ∗ hart_csrs ∗ own_context cur_ctx ∗
     (∀ ws' : list (mword 64),
-       ⌜tf_kernel_words_ok kroot ksp ws'⌝ -∗ tf_page (ud_tfp pt) ws' -∗ hart_csrs -∗
+       ⌜tf_kernel_words_ok kroot ksp ws'⌝ -∗ tf_page (ud_tfp pt) ws' -∗ hart_csrs -∗ own_context cur_ctx -∗
        usertrap_res_bare pt ksp).
 Proof. exact (ut_res_bare_tf_csrs_open SY.syscall_env pt ksp). Qed.
 
