iris/SpecUsertrap.v
@@ -515,10 +515,16 @@ Module Type USERTRAP_RES.
       usertrap_res_bare pt ksp -∗
       ∃ (kroot : mword 44) (ws : list (mword 64)),
         kpt_inv kroot ∗ ⌜tf_kernel_words_ok kroot ksp ws⌝ ∗
-        tf_page (ud_tfp pt) ws ∗ hart_csrs ∗
+        tf_page (ud_tfp pt) ws ∗ hart_csrs ∗ own_context cur_ctx ∗
         (∀ ws' : list (mword 64),
-           ⌜tf_kernel_words_ok kroot ksp ws'⌝ -∗ tf_page (ud_tfp pt) ws' -∗ hart_csrs -∗
+           ⌜tf_kernel_words_ok kroot ksp ws'⌝ -∗ tf_page (ud_tfp pt) ws' -∗ hart_csrs -∗ own_context cur_ctx -∗
            usertrap_res_bare pt ksp).
+
+  (* the token borrow -- [UsertrapRes.ut_res_bare_ctx_acc] *)
+  Parameter usertrap_res_bare_ctx :
+    forall `{!riscvGS Σ, !xv6G Σ, !bioslotG Σ, !fdslotG Σ, !fileG Σ, !irefslotG Σ, !pavG Σ} `{GEN : GenId} `{CID : CpuId} `{XI : CurCtx} (pt : uptd) (ksp : mword 64),
+      usertrap_res_bare pt ksp -∗
+      own_context cur_ctx ∗ (own_context cur_ctx -∗ usertrap_res_bare pt ksp).
 
   Parameter usertrap_res_tf_open :
     forall `{!riscvGS Σ, !xv6G Σ, !bioslotG Σ, !fdslotG Σ, !fileG Σ, !irefslotG Σ, !pavG Σ} `{GEN : GenId} `{CID : CpuId} `{XI : CurCtx} (pt : uptd) (ksp : mword 64),
@@ -527,8 +533,10 @@ Module Type USERTRAP_RES.
       usertrap_res_bare pt ksp -∗
       ∃ (kroot : mword 44) (ws : list (mword 64)),
         kpt_inv kroot ∗ ⌜tf_kernel_words_ok kroot ksp ws⌝ ∗ tf_page (ud_tfp pt) ws ∗
+        own_context cur_ctx ∗
         (∀ ws' : list (mword 64),
            ⌜tf_kernel_words_ok kroot ksp ws'⌝ -∗ tf_page (ud_tfp pt) ws' -∗
+         own_context cur_ctx -∗
            usertrap_res_bare pt ksp).
 End USERTRAP_RES.
 
